iris/ProofUserretClosed.v
@@ -263,7 +263,7 @@ Section UserretClosed.
     iApply wp_next_intro. iIntros (CID').
     rewrite /uservec_post.
     iIntros (pt' mf ms' usatp uepc sc' stval' mdv0 U2 sts2)
-      "%Huptpt' %Hround' %Hfdkept %Hpcret' %Hgprtie'
+      "%Huptpt' %Hround' %Hfdkept %Hfdecall %Hpcret' %Hgprtie'
        %Hpttf %Hmapwf %Hsatpr %Hnorm' %Hptwf' %Hmm %Hretms %Hacc'
        Hhs' Hpriv' Hms' Hmie' Hmdl' Hmenv' Hstvec' #Hsenv' Hsc' Hstval' Hsepc'
        Hupt' Hpc' Hgpr' Hures' #Hhw' #Hmin'".
